Add another toy example.

wand_demo/verif_list.v
@@ -3,7 +3,7 @@ Require Import wand_demo.wand_frame.
 Require Import wand_demo.list.
 Require Import wand_demo.list_lemmas.
 
-Module VerifHeadPointerSwitch.
+Module VerifHeadSwitch.
 
 Import ListHead.
   
@@ -19,7 +19,20 @@ Definition head_pointer_switch_spec :=
      LOCAL ()
      SEP   (listrep sh (y :: s) l; data_at sh tint (Vint x) p).
 
-Definition Gprog : funspecs := ltac:(with_library prog [ head_pointer_switch_spec ]).
+Definition head_head_switch_spec :=
+ DECLARE _head_head_switch
+  WITH sh : share, l1: val, l2: val, h1: int, t1: list int, h2: int, t2: list int
+  PRE [ _l1 OF (tptr t_struct_list) , _l OF (tptr t_struct_list)]
+     PROP  (writable_share sh)
+     LOCAL (temp _l1 l1; temp _l2 l2)
+     SEP   (listrep sh (h1 :: t1) l1; listrep sh (h2 :: t2) l2)
+  POST [ tvoid ]
+     PROP  ()
+     LOCAL ()
+     SEP   (listrep sh (h2 :: t1) l1; listrep sh (h1 :: t2) l2).
+
+Definition Gprog : funspecs :=
+  ltac:(with_library prog [ head_pointer_switch_spec; head_head_switch_spec]).
 
 (* TODO: try use sep_apply in this proof instead of cancel, sepcon_comm. *)
 Lemma body_head_pointer_switch: semax_body Vprog Gprog f_head_pointer_switch head_pointer_switch_spec.
@@ -30,7 +43,7 @@ Proof.
       (field_at sh t_struct_list [StructField _head] (Vint y) l -* listrep sh (y :: s) l)).
     {
       entailer!.
-      apply wf_intro_list_head.
+      apply wand_frame_intro_list_head.
     }
   Intros. freeze [1] Fr.  
     forward. (* h = l -> head; *)
@@ -40,10 +53,39 @@ Proof.
   thaw Fr.
   forward. (* return *)
   cancel.
-  rewrite sepcon_comm. apply wf_elim.
+  rewrite sepcon_comm. apply wand_frame_elim.
 Qed.
 
-End VerifHeadPointerSwitch.
+Lemma body_head_head_switch: semax_body Vprog Gprog f_head_head_switch head_head_switch_spec.
+Proof.
+  start_function.
+  replace_SEP 0
+    (field_at sh t_struct_list [StructField _head] (Vint h1) l1 *
+      (field_at sh t_struct_list [StructField _head] (Vint h2) l1 -* listrep sh (h2 :: t1) l1)).
+    {
+      entailer!.
+      apply wand_frame_intro_list_head.
+    }
+  replace_SEP 1
+    (field_at sh t_struct_list [StructField _head] (Vint h2) l2 *
+      (field_at sh t_struct_list [StructField _head] (Vint h1) l2 -* listrep sh (h1 :: t2) l2)).
+    {
+      entailer!.
+      apply wand_frame_intro_list_head.
+    }
+  Intros. freeze [1; 3] Fr.  
+    forward. (* h1 = l1 -> head; *)
+    forward. (* h2 = l2 -> head; *)
+    forward. (* l1 -> head = h2; *)
+    forward. (* l2 -> head = h1; *)
+  thaw Fr.
+  forward. (* return *)
+  rewrite sepcon_assoc.
+  eapply derives_trans; [apply sepcon_derives; [apply wand_frame_hor | apply derives_refl] |].
+  rewrite sepcon_comm. apply wand_frame_elim.
+Qed.
+
+End VerifHeadSwitch.
 (*
 
 Definition append_spec (_append: ident) :=
